rework: definitions need to introduce axioms!
Axioms are the things that constrain interpretations when we consider
entailment. So, the theorems that come out of the definitional
principles need to be treated as axioms, since otherwise there's no
reason an interpretation can interpret the new constant as something
unintended.

With this change, the soundness proof comes through easily.

But, consistency is going to be difficult! Because for consistency we
need to know that the axioms are consistent. This will require some
extra proofs...

hol-light/stateful/holSyntaxScript.sml
@@ -331,10 +331,22 @@ val terms_of_def_def = Define`
   (* Axioms *)
 val axioms_of_def_def = Define`
   (axioms_of_def (NewAxiom prop) = [prop]) ∧
+  (axioms_of_def (ConstSpec eqs prop) =
+   let ilist = MAP (λ(s,t). let ty = typeof t in (Const s ty,Var s ty)) eqs in
+     [VSUBST ilist prop]) ∧
+  (axioms_of_def (TypeDefn name pred abs_name rep_name) =
+    let abs_type = Tyapp name (MAP Tyvar (STRING_SORT (tvars pred))) in
+    let rep_type = domain (typeof pred) in
+    let abs = Const abs_name (Fun rep_type abs_type) in
+    let rep = Const rep_name (Fun abs_type rep_type) in
+    let a = Var "a" abs_type in
+    let r = Var "r" rep_type in
+      [Comb abs (Comb rep a) === a;
+       Comb pred r === (Comb rep (Comb abs r) === r)]) ∧
   (axioms_of_def _ = [])`
 val _ = Parse.overload_on("axioms",``λctxt. FLAT (MAP axioms_of_def ctxt)``)
 
-val _ = export_rewrites["types_of_def_def","consts_of_def_def","terms_of_def_def","axioms_of_def_def"]
+val _ = export_rewrites["types_of_def_def","consts_of_def_def","terms_of_def_def"]
 
 (* Good types/terms in context *)
 
@@ -454,8 +466,7 @@ val (proves_rules,proves_ind,proves_cases) = xHol_reln"proves"`
    (∀s. MEM s (MAP FST eqs) ⇒ s ∉ (FDOM (consts ctxt))) ∧
    ALL_DISTINCT (MAP FST eqs) ∧
    ((ctxt, asl) |- p ∨
-    (let ilist = MAP (λ(s,t). let ty = typeof t in (Const s ty,Var s ty)) eqs in
-       (asl,p) = ([],VSUBST ilist prop)))
+    (asl = [] ∧ MEM p (axioms_of_def (ConstSpec eqs prop))))
    ⇒ ((ConstSpec eqs prop)::ctxt, asl) |- p) ∧
 
   (* new_type *)
@@ -464,23 +475,14 @@ val (proves_rules,proves_ind,proves_cases) = xHol_reln"proves"`
    ⇒ ((NewType name arity)::ctxt, asl) |- p) ∧
 
   (* new_type_definition *)
-  ((abs_type = Tyapp name (MAP Tyvar (STRING_SORT (tvars pred)))) ∧
-   (ctxt, []) |- Comb pred witness ∧
+  ((ctxt, []) |- Comb pred witness ∧
    CLOSED pred /\ pred has_type (Fun rep_type Bool) ∧
    name ∉ (FDOM (types ctxt)) ∧
    abs ∉ (FDOM (consts ctxt)) ∧
    rep ∉ (FDOM (consts ctxt)) ∧
    abs ≠ rep ∧
-   ((ctxt, asl) |- p  ∨
-    ((asl,p) = ([],
-       Comb (Const abs (Fun rep_type abs_type))
-              (Comb (Const rep (Fun abs_type rep_type))
-                    (Var x abs_type)) === Var x abs_type)) ∨
-    ((asl,p) = ([],
-       Comb t (Var x rep_type) ===
-          Comb (Const rep (Fun abs_type rep_type))
-               (Comb (Const abs (Fun rep_type abs_type))
-                     (Var x rep_type)) === Var x rep_type)))
+   ((ctxt, asl) |- p ∨
+    (asl = [] ∧ MEM p (axioms_of_def (TypeDefn name pred abs rep))))
    ⇒ ((TypeDefn name pred abs rep)::ctxt, asl) |- p)`
 
 (*
